examples/riscv/mod2/mod2_symb_transfScript.sml
@@ -19,8 +19,8 @@ val _ = new_theory "mod2_symb_transf";
 val init_addr_tm = (snd o dest_eq o concl) mod2_init_addr_def;
 val end_addr_tm = (snd o dest_eq o concl) mod2_end_addr_def;
 
-val bspec_pre_tm = ``bspec_mod2_pre pre_x10``;
-val bspec_post_tm = ``bspec_mod2_post pre_x10``;
+val bspec_pre_tm = (lhs o snd o strip_forall o concl) bspec_mod2_pre_def;
+val bspec_post_tm = (lhs o snd o strip_forall o concl) bspec_mod2_post_def;
 
 (* ------------------------------- *)
 (* BIR symbolic execution analysis *)
@@ -28,7 +28,8 @@ val bspec_post_tm = ``bspec_mod2_post pre_x10``;
 
 val bspec_cont_thm =
  bir_symb_transfer init_addr_tm end_addr_tm bspec_pre_tm bspec_post_tm
-  bir_mod2_prog_def mod2_birenvtyl_def bspec_mod2_pre_def bspec_mod2_post_def mod2_prog_vars_def
+  bir_mod2_prog_def mod2_birenvtyl_def
+  bspec_mod2_pre_def bspec_mod2_post_def mod2_prog_vars_def
   mod2_symb_analysis_thm mod2_bsysprecond_thm mod2_prog_vars_thm;
 
 Theorem bspec_cont_mod2:
